src/Language/PlutusIR/Semantics/Dynamic/Bigstep/Examples/AddInteger.v
@@ -14,11 +14,12 @@ Local Open Scope string_scope.
 Definition Ty_int : Ty := Ty_Builtin (Some (TypeIn DefaultUniInteger)).
 Definition int_to_int : Ty := Ty_Fun Ty_int Ty_int.
 
-Example test_addInteger : forall x,
+Example test_addInteger : forall x, exists k,
   Apply (LamAbs x int_to_int (Apply (Var x) (constInt 17))) (Apply (Builtin AddInteger) (constInt 3))
-  ==> constInt 20.
+  =[k]=> constInt 20.
 Proof.
   intros.
+  eexists.
   eapply E_Apply.
   - apply E_LamAbs.
   - eapply E_ApplyBuiltin1.
